chore(*) : finishes proof for updated IS_S2

example.lean
@@ -1,38 +1,79 @@
 import common hoare.basic big_step.basic
 
-def IS_S2 (I : ℕ): stmt :=
-    stmt.ite (λ s, s "Conn" ∧ s "AuthConn" ∧ ¬ s "BuffChng")
-        (stmt.assign "I" (λ s, (I = 1))) (stmt.skip)
+lemma le_of_lt_succ {a b : ℕ} : a < b → (nat.succ a) ≤ b := sorry
 
-lemma correct {Conn AuthConn BuffChng: Prop} (I : ℕ) (init : Conn ∧ AuthConn ∧ BuffChng) :
-    {* λ s, s "Conn" = Conn ∧ s "AuthConn" = AuthConn ∧ s "BuffChng" = ¬ BuffChng ∧ s "I" = (I = 0) *}
-    IS_S2 I
-    {* λ s, s "Conn" = Conn ∧ s "AuthConn" = AuthConn ∧ s "BuffChng" = ¬ BuffChng ∧ (s "I" → (0 ≤ I)) *} :=
+def IS_S2 {BuffChng : Prop} (Len Cap I: ℕ) : stmt :=
+    stmt.ite (λ s, (s "I" → I ≤ Cap) ∧ s "Conn" ∧ s "AuthConn" ∧ ¬ s "BuffChng")
+        ((stmt.assign "I" (λ s, (I = 1))) ;; (stmt.assign "Cap" (λ s, (Cap = Len))) ;; (stmt.assign "BuffChng" (λ s, BuffChng)))
+        (stmt.skip)
+
+lemma IS_S2_correct {Conn AuthConn BuffChng : Prop} (Len Cap I : ℕ) (Buff BuffOut : list ℕ) (props : Conn ∧ AuthConn ∧ BuffChng) :
+    {* λ s, s "Conn" = Conn ∧ s "AuthConn" = AuthConn ∧ s "BuffChng" = ¬ BuffChng ∧ 0 < Len ∧ s "Cap" = (Cap = Len) ∧ s "I" = (I = 0) *}
+    @IS_S2 BuffChng Len Cap I
+    {* λ s, s "Conn" = Conn ∧ s "AuthConn" = AuthConn ∧ s "BuffChng" = BuffChng ∧ 0 < Len ∧ (s "Cap" → (Cap = Len)) ∧ (s "Cap" → s "I" → (I ≤ Cap)) *} :=
 begin
     rw IS_S2,
     apply partial_hoare.ite_true_intro,
     {
         intros s hS,
-        rw [hS.1, hS.2.1, hS.2.2.1],
-        cc,
-    },
-    {
-        apply partial_hoare.assign_intro',
-        intros s hS,
         cases hS with h₁ h₂,
         cases h₂ with h₃ h₄,
         cases h₄ with h₅ h₆,
+        cases h₆ with h₇ h₈,
+        rw [h₈.right, h₁, h₃, h₅],
         split,
-            rw scope.update_apply_ne "I" "Conn" (I = 1) s,
-            exact h₁,
+            intro hI,
+            rw hI,
+            exact dec_trivial,
         split,
-            rw scope.update_apply_ne "I" "AuthConn" (I = 1) s,
-            exact h₃,
+            exact props.1,
         split,
-            rw scope.update_apply_ne "I" "BuffChng" (I = 1) s,
-            exact h₅,
-        rw scope.update_apply,
-        intro hI,
-        exact dec_trivial,
+            exact props.2.1,
+        apply non_contradictory_intro,
+        exact props.2.2,
+    },
+    {
+        apply partial_hoare.comp_intro,
+        {
+            apply partial_hoare.assign_intro_right,
+        },
+        {
+            apply partial_hoare.comp_intro,
+            {
+                apply partial_hoare.assign_intro_right,
+            },
+            {
+                apply partial_hoare.assign_intro',
+                intros s ht₀,
+                have t₀ : Prop := Cap = Len,
+                cases ht₀ with t₀ ht₀_1,
+                cases ht₀_1 with ht₀_1 hCap,
+                cases ht₀_1 with t₀_1 hS,
+                simp at hS,
+                cases hS with h₁ h₂,
+                cases h₁ with h₁ h₃,
+                cases h₃ with h₃ h₄,
+                cases h₄ with h₄ h₅,
+                cases h₅ with h₅ h₆,
+                cases h₆ with h₆ h₇,
+                simp,
+                split,
+                    exact h₁,
+                split,
+                    exact h₃,
+                split,
+                    exact h₅,
+                split,
+                    intro hsCap,
+                    rw hCap at hsCap,
+                    exact hsCap,
+                rw h₂,
+                rw hCap,
+                intros hCap hI,
+                rw [hI, hCap],
+                apply le_of_lt_succ,
+                exact h₅,
+            }
+        }
     }
 end
